read I believe.

PerryHomework2.v
@@ -110,7 +110,18 @@ Theorem popINVARIANT1: forall n : nat, forall ns : NatStack, pop (push n ns) = n
 Theorem topPOST1 : forall ns:NatStack, forall n :nat, top (push n ns) = Value n .
  Proof. intros. simpl. reflexivity. Qed.
 Theorem topINVARIANT1 : forall ns:NatStack, forall n : nat, (top (push n ns)) = Value n -> ns = ns.
- Proof. intros. reflexivity. Qed. 
+ Proof. intros. reflexivity. Qed.
+
+Theorem isEmptyPOST1 : forall s : NatStack, isEmpty s = true <-> s = Empty.
+Proof. intros. split. induction s.  simpl. symmetry. reflexivity. 
+simpl. discriminate.
+intros. rewrite H.  simpl.  reflexivity. Qed. 
+Theorem isEmptyPOST2 : forall s : NatStack, isEmpty s = false <-> s <> Empty.
+Proof. intros. split. intros. destruct s. discriminate.
+simpl. discriminate. intros. unfold isEmpty. destruct s. elim H.  reflexivity. 
+reflexivity.  Qed. 
+Theorem isEmptyINVARIANT1 : forall s : NatStack, isEmpty s = true /\ isEmpty s = false -> s = s.
+Proof. intros.  reflexivity. Qed. 
 
 Definition s1 := push 1 (push 2 (push 3 Empty)).
 Definition emp := Empty .
@@ -126,40 +137,201 @@ End problem1.
 
 Module problem2. 
 
-Inductive SC : Type :=
-| Value : nat -> SC
-| Unknown : SC.
+Inductive SC (T :Type): Type :=
+| Value : T -> SC T
+| Unknown : SC T.
 
-Inductive NatStack : Type :=
-| Empty : NatStack
-| Add : nat -> NatStack -> NatStack.
+Inductive Stack (T:Type) : Type :=
+| Empty : Stack T
+| Add : T -> Stack T -> Stack T.
+
+Eval compute in Add nat 4 (Empty nat).
 
 
-Definition push(sc:SC) (ns : NatStack) : NatStack :=
-   match sc with 
-    | Unknown => ns 
-    | Value n => Add n ns
+Definition push {T:Type} (t:T) (st : Stack T) : Stack T:=
+   Add T t st.
+
+Definition pop {T:Type} (s : Stack T) : Stack T :=
+   match s with
+    | Empty => Empty T 
+    | Add _ s' => s' 
    end.
 
-Definition pop(ns : NatStack) : NatStack :=
-   match ns with
-    | Empty => Empty 
-    | Add _ ns' => ns' 
-   end.
-
-Definition top (ns:NatStack):SC :=
-   match ns with 
-    | Empty => Unknown
-    | Add x _ => Value x
+Definition top {T:Type} (s:Stack T): SC T :=
+   match s with 
+    | Empty => Unknown T
+    | Add x _ => Value T x
    end. 
 
-Definition isEmpty(ns : NatStack) : bool :=
-   match ns with 
+Definition isEmpty {T:Type} (s : Stack T) : bool :=
+   match s with 
+    | Empty => true
+    | Add _ _ => false
+   end.
+
+Theorem pushPOST1 : forall (T:Type), forall t :T, forall s:Stack T, push t s <> Empty T.
+  Proof. intros. unfold push. discriminate. Qed.
+Theorem pushPOST2 : forall (T:Type), forall t : T, forall s: Stack T, top (push t s) = Value T t.
+  Proof. intros.  simpl. reflexivity. Qed.
+Theorem pushINVARIANT1 : forall (T:Type), forall t :T, forall s : Stack T, pop (push t s) = s.
+  Proof. intros.  simpl. reflexivity. Qed.
+
+
+Fixpoint size {T:Type} (s:Stack T) : nat :=
+  match s with 
+    | Empty => O
+    | Add _ ns' => S (size ns')
+  end.
+
+Theorem popPost1 : forall T:Type, forall t:T, forall s: Stack T, s <>Empty T -> size s = S (size (pop s)).
+  Proof. intros. induction s. elim H. reflexivity.
+    simpl. reflexivity. Qed.
+Theorem popPost2 : forall T:Type, forall t:T, forall s:Stack T, top s = Value T t <-> Value T t = top (pop (push t s)).
+ Proof.  split. simpl. intros. elim H. reflexivity. 
+         simpl. symmetry. elim H. reflexivity. Qed.
+Theorem popINVARIANT1: forall T:Type, forall t : T, forall s : Stack T, pop (push t s) = s.
+ Proof. apply pushINVARIANT1. Qed.
+
+Theorem topPOST1 : forall T:Type, forall s:Stack T,  forall t :T, top (push t s) = Value T t .
+ Proof. intros. simpl. reflexivity. Qed.
+Theorem topINVARIANT1 : forall T:Type, forall s:Stack T, forall t : T, (top (push t s)) = Value T t -> s = s.
+ Proof. intros. reflexivity. Qed.
+
+Theorem isEmptyPOST1 : forall T : Type, 
+                       forall s : Stack T, 
+                       isEmpty s = true <-> s = Empty T.
+Proof. intros. split. induction s.  simpl. symmetry. reflexivity. 
+simpl. discriminate.
+intros. rewrite H.  simpl.  reflexivity. Qed. 
+Theorem isEmptyPOST2 : forall T : Type,
+                       forall s : Stack T, 
+                       isEmpty s = false <-> s <> Empty T.
+Proof. intros. split. intros. destruct s. discriminate.
+simpl. discriminate. intros. unfold isEmpty. destruct s. elim H.  reflexivity. 
+reflexivity.  Qed. 
+Theorem isEmptyINVARIANT1 : forall T: Type, 
+                            forall s : Stack T, 
+                            isEmpty s = true /\ isEmpty s = false -> s = s.
+Proof. intros.  reflexivity. Qed. 
+(*3*) 
+Example prob2_3 : forall T:Type, forall x y : T, (pop (pop (push y (push x (Empty T))))) = Empty T.
+Proof.  intros. simpl. reflexivity. Defined.
+(* the two pops come after 2 pushes, so we have never "reached too far". We end up with the empty stack that was our base.*)
+Example prob2_4 : forall T:Type, forall x: T, (pop (pop (push x (Empty T)))) = Empty T.
+Proof.  intros. simpl. reflexivity. Defined.
+(* We have defined pop such that popping the empty stack will simply result in another
+   empty stack. This is not safe becase we have allowed for an implementer to call pop
+   on an empty stack without conveying the information that the stack was already empty.
+   Basically, if your code ever calls pop on empty, you screwed up somewhere, and right
+   now our implementation is totally cool with you calling pop on empty-- I'll just give
+   you another empty. *)
+End problem2. 
+
+
+Module problem3. 
+
+Inductive Stack (T:Type) : Type :=
+| Empty : Stack T
+| Add : T -> Stack T -> Stack T.
+
+Definition push {T:Type} (t:T) (st : Stack T) : Stack T:=
+   Add T t st.
+
+Definition pop {T:Type} (s : Stack T) (p : s <> (Empty T)) : Stack T.
+Proof. destruct s as [|e s']. elim p.  reflexivity.  exact (s'). Defined.
+
+Definition top {T:Type} (s:Stack T) (p:s <> Empty T): T.
+Proof. destruct s. elim p. reflexivity. exact t. Defined.
+
+Definition s1 := (Add nat 3 (Empty nat)).
+Definition s1p : s1 <> Empty nat.
+Proof. discriminate. Defined.
+
+Eval compute in top s1 s1p.
+
+Definition isEmpty {T:Type} (s : Stack T) : bool :=
+   match s with 
     | Empty => true
     | Add _ _ => false
    end.
 
 
+Theorem pushPOST1 : forall (T:Type), forall t :T, forall s:Stack T, push t s <> Empty T.
+  Proof. intros. unfold push. discriminate. Qed.
+Theorem pushPOST2 : forall (T:Type), forall t : T, forall s: Stack T, forall p : (push t s) <> Empty T, top (push t s) p = t .
+  Proof. intros.  simpl. reflexivity. Qed.
+Theorem pushINVARIANT1 : forall (T:Type), forall t :T, forall s : Stack T,forall p : (push t s) <> Empty T, pop (push t s) p= s.
+  Proof. intros.  simpl. reflexivity. Qed.
 
 
+Fixpoint size {T:Type} (s:Stack T) : nat :=
+  match s with 
+    | Empty => O
+    | Add _ ns' => S (size ns')
+  end.
 
+Theorem popPost1 : forall T:Type, forall t:T, forall s: Stack T, forall p : (s) <> Empty T, size s = S (size (pop s p)).
+  Proof. intros. induction s. elim p. reflexivity.
+    simpl. reflexivity. Qed.
+Theorem popPost2 : forall T:Type, 
+                   forall t:T, 
+                   forall s:Stack T,
+                   forall p : (push t s) <> Empty T,
+                   forall p2 : (s) <> Empty T,     
+                   top s p2 = t <->  t = top (pop (push t s) p) p2.
+ Proof.  split. simpl. intros. elim H. reflexivity. 
+         simpl. symmetry. elim H. reflexivity. Qed.
+Theorem popINVARIANT1: forall T:Type, 
+                       forall t : T, 
+                       forall s : Stack T, 
+                       forall p : (push t s) <> Empty T,
+                       pop (push t s) p = s.
+ Proof. apply pushINVARIANT1. Qed.
+
+Theorem topPOST1 : forall T:Type, 
+                   forall s:Stack T,  
+                   forall t :T, 
+                   forall p : (push t s) <> Empty T, 
+                   top (push t s) p = t .
+ Proof. intros. simpl. reflexivity. Qed.
+
+Theorem topINVARIANT1 : forall T:Type, 
+                        forall s:Stack T, 
+                        forall t : T, 
+                        forall p : (push t s) <> Empty T,
+                        (top (push t s)) p = t -> s = s.
+ Proof. intros. reflexivity. Qed.
+
+Theorem isEmptyPOST1 : forall T : Type, 
+                       forall s : Stack T, 
+                       isEmpty s = true <-> s = Empty T.
+Proof. intros. split. induction s.  simpl. symmetry. reflexivity. 
+simpl. discriminate.
+intros. rewrite H.  simpl.  reflexivity. Qed. 
+Theorem isEmptyPOST2 : forall T : Type,
+                       forall s : Stack T, 
+                       isEmpty s = false <-> s <> Empty T.
+Proof. intros. split. intros. destruct s. discriminate.
+simpl. discriminate. intros. unfold isEmpty. destruct s. elim H.  reflexivity. 
+reflexivity.  Qed. 
+Theorem isEmptyINVARIANT1 : forall T: Type, 
+                            forall s : Stack T, 
+                            isEmpty s = true /\ isEmpty s = false -> s = s.
+Proof. intros.  reflexivity. Qed. 
+
+Definition constructable (T:Type) (s :Stack T) : Prop := True.
+ 
+Example neverEver : forall T:Type,
+                    forall x : T,
+                    forall s: Stack T,
+                    forall p1 : (push x (Empty T)) <> Empty T,
+                    forall p2 : pop (push x (Empty T)) p1 <> Empty T,
+                    (constructable T (pop (pop (push x (Empty T)) p1) p2)) -> False.
+Proof. intros. simpl in p2.  elim p2.  reflexivity. Qed.
+(* The above proves that calling (pop (pop (push x (Empty T)))) is an impossible term
+   to construct. Mainly, note that it needs a proof of the type of 'p2', which simplifes to 
+   proving that Empty <> Empty. If you can do that, you've successfully proven False.
+   To summarize, the above example shows that constructing a term of the form (pop (pop push _ empty)))
+   implies False, an impossibility. *)
+End problem3.
+   
